bir_envScript.sml, bir_expScript.sml, bir_immScript.sml updated with total map as variable environment. bir_typing_expScript.sml WIP

src/theory/bir/bir_envScript.sml
@@ -23,7 +23,8 @@ SIMP_TAC std_ss [bir_var_type_def, bir_var_name_def, bir_var_t_11]
 
 val _ = Datatype `bir_var_environment_t =
    BEnv (string -> (bir_val_k_t))`;
-val bir_var_environment_t_11 = DB.fetch "-" "bir_var_environment_t_11";
+val bir_var_environment_t_11 =
+  DB.fetch "-" "bir_var_environment_t_11";
 
 (* Empty environment *)
 (* TODO: What now? *)
@@ -45,26 +46,23 @@ val bir_env_lookup_def = Define `
   (bir_env_lookup varname (BEnv env) = env varname)`;
 
 val bir_env_update_def = Define `
-  (bir_env_update varname vo ty (BEnv env) =
-    if (ty <> type_of_bir_kval vo)
+  (bir_env_update varname vo vartype (BEnv env) =
+    if (vartype <> type_of_bir_kval vo)
     then NONE
     else SOME (BEnv ((varname =+ vo) env))
   )`;
 
 val bir_env_lookup_UPDATE = store_thm ("bir_env_lookup_UPDATE",
-``!vn vn' vo env.
-  bir_env_lookup vn (BEnv ((vn' =+ vo) env)) =
-   (if (vn' = vn)
-    then vo
-    else bir_env_lookup vn (BEnv env))``,
+  ``!vn vn' vo env.
+    bir_env_lookup vn (BEnv ((vn' =+ vo) env)) =
+     (if (vn' = vn)
+      then vo
+      else bir_env_lookup vn (BEnv env))``,
 
 SIMP_TAC std_ss [bir_env_lookup_def, UPDATE_def]
 );
 
-(* Note: After introduction of the total map, this now checks the
- *       type of the value stored using type_of_bir_kval, instead of
- *       checking the type stored in the tuple.
- *       An alternative could be to do no checking at all. *)
+
 val bir_env_lookup_type_def = Define `
   bir_env_lookup_type var_name env =
     type_of_bir_kval (bir_env_lookup var_name env)`;
@@ -76,35 +74,55 @@ val bir_env_check_type_def = Define `
       bir_var_type var
     )`;
 
-
+(* Note design choice: BVal_Unknown is returned upon explicit type
+ * disagreement between stored and looked-up variable. *)
 val bir_env_read_def = Define `bir_env_read v env =
-  bir_env_lookup (bir_var_name v) env`;
+  if (bir_env_check_type v env)
+  then BVal_Known (bir_env_lookup (bir_var_name v) env)
+  else BVal_Unknown`;
 
-(* TODO: This checks the type of the stored value - if types do
- *       not agree, then keep on checking. *)
+
 val bir_env_read_UPDATE = store_thm ("bir_env_read_UPDATE",
-``!v vn vo env.
-  bir_env_read v (BEnv ((vn =+ vo) env)) =
-   (if (bir_var_name v = vn) then (
-      if (type_of_bir_kval vo = bir_var_type v) then
-         vo
-      else bir_env_read v (BEnv env))
- else bir_env_read v (BEnv env))``,
+  ``!v vn vo env.
+    bir_env_read v (BEnv ((vn =+ vo) env)) =
+      (if (bir_var_name v = vn)
+       then (if (type_of_bir_kval vo = bir_var_type v)
+             then BVal_Known vo
+             else BVal_Unknown
+            )
+       else bir_env_read v (BEnv env)
+      )``,
 
 REPEAT STRIP_TAC >>
 SIMP_TAC std_ss [bir_env_read_def, bir_env_lookup_UPDATE] >>
-Cases_on `bir_var_name v = vn` >> ASM_SIMP_TAC std_ss [] >>
-Cases_on `vo` >> SIMP_TAC std_ss [pairTheory.pair_case_thm]
+Cases_on `bir_var_name v = vn` >> (
+  FULL_SIMP_TAC std_ss [type_of_bir_kval_def,
+			bir_env_check_type_def,
+			bir_env_lookup_type_def,
+                        bir_env_lookup_def,
+			combinTheory.UPDATE_APPLY]
+)
 );
 
-val bir_env_read_NEQ_UNKNOWN = store_thm ("bir_env_read_NEQ_UNKNOWN",
-``!var env v.
-(v <> BVal_Unknown) ==>
-((bir_env_read var env = v) <=> (bir_env_lookup (bir_var_name var) env = SOME (bir_var_type var, SOME v)))``,
+(* Note: Gains a new antecedent from no longer having type in the
+ * returning tuple. *)
+val bir_env_read_NEQ_UNKNOWN =
+  store_thm ("bir_env_read_NEQ_UNKNOWN",
+  ``!var env v.
+    (type_of_bir_kval v = bir_var_type var) ==>
+    ((bir_env_read var env = BVal_Known v) <=>
+     (bir_env_lookup (bir_var_name var) env =
+        v
+     )
+    )``,
 
-REPEAT GEN_TAC >>
-SIMP_TAC std_ss [bir_env_read_def] >>
-REPEAT CASE_TAC);
+REPEAT STRIP_TAC >>
+SIMP_TAC std_ss [bir_env_read_def,
+                 bir_env_check_type_def,
+                 bir_env_lookup_type_def] >>
+REPEAT CASE_TAC >>
+METIS_TAC []
+);
 
 val bir_env_write_def = Define `bir_env_write v va env =
   if (bir_env_check_type v env)
@@ -113,18 +131,24 @@ val bir_env_write_def = Define `bir_env_write v va env =
 
 
 val bir_env_write_WrongVal = store_thm ("bir_env_write_WrongVal",
-  ``!v va env. (type_of_bir_kval va <> SOME (bir_var_type v)) ==>
-               (bir_env_write v va env = NONE)``,
+  ``!v va env.
+    (type_of_bir_kval va <> bir_var_type v) ==>
+    (bir_env_write v va env = NONE)``,
 
 REPEAT GEN_TAC >> Cases_on `env` >>
-SIMP_TAC std_ss [bir_env_write_def, bir_env_check_type_def,
-  bir_env_update_def]);
+SIMP_TAC std_ss [bir_env_write_def,
+                 bir_env_check_type_def,
+                 bir_env_lookup_type_def, 
+                 bir_env_update_def]
+);
 
-val bir_env_update_is_well_typed_env = store_thm ("bir_env_update_is_well_typed_env",
-``!env env' varname vo ty.
-    (bir_is_well_typed_env env /\
-    (bir_env_update varname vo ty env = SOME env')) ==>
-    bir_is_well_typed_env env'``,
+(* Deprecated...
+val bir_env_update_is_well_typed_env =
+  store_thm ("bir_env_update_is_well_typed_env",
+  ``!env env' varname vo ty.
+      (bir_is_well_typed_env env /\
+      (bir_env_update varname vo ty env = SOME env')) ==>
+      bir_is_well_typed_env env'``,
 
 Cases >>
 SIMP_TAC std_ss [bir_env_update_def, bir_is_well_typed_env_def] >>
@@ -133,8 +157,11 @@ ConseqConv.CONSEQ_REWRITE_TAC ([FEVERY_STRENGTHEN_THM], [], []) >>
 ASM_SIMP_TAC std_ss [] >>
 Cases_on `vo` >> (
   FULL_SIMP_TAC std_ss []
-));
+)
+);
+*)
 
+(* Deprecated...
 val bir_env_write_is_well_typed_env = store_thm ("bir_env_write_is_well_typed_env",
 ``!env env' v va.
     (bir_is_well_typed_env env /\
@@ -142,10 +169,13 @@ val bir_env_write_is_well_typed_env = store_thm ("bir_env_write_is_well_typed_en
     bir_is_well_typed_env env'``,
 
 SIMP_TAC std_ss [bir_env_write_def] >>
-METIS_TAC[bir_env_update_is_well_typed_env]);
+METIS_TAC[bir_env_update_is_well_typed_env]
+);
+*)
 
-
-val bir_is_well_typed_env_lookup = store_thm ("bir_is_well_typed_env_lookup",
+(* Deprecated...
+val bir_is_well_typed_env_lookup =
+  store_thm ("bir_is_well_typed_env_lookup",
   ``!env vn ty v. bir_is_well_typed_env env ==>
                   (bir_env_lookup vn env = SOME (ty, SOME v)) ==>
                   (type_of_bir_val v = SOME ty)``,
@@ -155,145 +185,187 @@ rename1 `BEnv f` >>
 SIMP_TAC (std_ss++QI_ss) [bir_env_lookup_def, FEVERY_ALL_FLOOKUP] >>
 REPEAT STRIP_TAC >>
 Q.PAT_X_ASSUM `!k. _` (MP_TAC o Q.SPEC `vn`) >>
-ASM_SIMP_TAC std_ss []);
+ASM_SIMP_TAC std_ss []
+);
+*)
 
+(* Old name: bir_is_well_typed_env_read *)
 
-val bir_is_well_typed_env_read = store_thm ("bir_is_well_typed_env_read",
-  ``!env v ty r. bir_is_well_typed_env env ==>
-                 (bir_env_read v env = r) ==>
-                 (r <> BVal_Unknown) ==>
-                 (type_of_bir_val r = SOME (bir_var_type v))``,
+val bir_env_read_type =
+  store_thm ("bir_env_read_type",
+  ``!env v ty r.
+      (bir_env_read v env = r) ==>
+      (r <> BVal_Unknown) ==>
+      (type_of_bir_val r = SOME (bir_var_type v))``,
 
 SIMP_TAC std_ss [bir_env_read_def] >>
 REPEAT GEN_TAC >>
-REPEAT CASE_TAC >> FULL_SIMP_TAC std_ss [type_of_bir_val_def, pairTheory.pair_case_thm] >>
-METIS_TAC[bir_is_well_typed_env_lookup]);
+REPEAT CASE_TAC >>
+FULL_SIMP_TAC std_ss [type_of_bir_val_def,
+                      bir_env_check_type_def,
+                      bir_env_lookup_type_def]
+);
 
 
 val bir_env_read_EQ_Unknown = store_thm ("bir_env_read_EQ_Unknown",
-  ``!v env. bir_is_well_typed_env env ==> (
-       (bir_env_read v env = BVal_Unknown) <=> (!r. (bir_env_lookup (bir_var_name v) env <> (SOME (bir_var_type v, SOME r)))))``,
+  ``!v env.
+        (bir_env_read v env = BVal_Unknown) <=>
+          (!kv.
+            (type_of_bir_kval kv = bir_var_type v) ==>
+            (bir_env_lookup (bir_var_name v) env <>
+              kv
+            )
+          )``,
 
 REPEAT GEN_TAC >>
 SIMP_TAC std_ss [bir_env_read_def] >>
-REPEAT CASE_TAC >>
-STRIP_TAC >>
-rename1 `r = BVal_Unknown` >>
-`type_of_bir_val r = SOME (bir_var_type v)` by METIS_TAC[bir_is_well_typed_env_lookup] >>
-STRIP_TAC >>
-FULL_SIMP_TAC std_ss [type_of_bir_val_def]);
-
-
-
-
+REPEAT CASE_TAC >> (
+  FULL_SIMP_TAC std_ss [bir_env_lookup_type_def,
+			bir_env_check_type_def]
+)
+);
+(*
+(* All varnames are bound in a total map, so... *)
 val bir_env_varname_is_bound_def = Define `
   (bir_env_varname_is_bound (BEnv env) var = (var IN FDOM env))`;
 
-val bir_env_varname_is_bound_ALT_DEF = store_thm ("bir_env_varname_is_bound_ALT_DEF",
-  ``!var env. bir_env_varname_is_bound env var <=> IS_SOME (bir_env_lookup_type var env)``,
+val bir_env_varname_is_bound_ALT_DEF =
+  store_thm ("bir_env_varname_is_bound_ALT_DEF",
+  ``!var env.
+      bir_env_varname_is_bound env var <=>
+        IS_SOME (bir_env_lookup_type var env)``,
 
 Cases_on `env` >> (
-  SIMP_TAC (std_ss++boolSimps.LIFT_COND_ss) [bir_env_varname_is_bound_def,
-    bir_env_lookup_type_def, bir_env_lookup_def, FLOOKUP_DEF]
-));
+  SIMP_TAC (std_ss++boolSimps.LIFT_COND_ss)
+           [bir_env_varname_is_bound_def,
+            bir_env_lookup_type_def, bir_env_lookup_def,
+            FLOOKUP_DEF]
+)
+);
 
-val bir_env_varname_is_bound_ALT2_DEF = store_thm ("bir_env_varname_is_bound_ALT2_DEF",
-  ``!var env. bir_env_varname_is_bound env var <=> IS_SOME (bir_env_lookup var env)``,
+val bir_env_varname_is_bound_ALT2_DEF =
+  store_thm ("bir_env_varname_is_bound_ALT2_DEF",
+  ``!var env.
+      bir_env_varname_is_bound env var <=>
+        IS_SOME (bir_env_lookup var env)``,
 
-SIMP_TAC std_ss [bir_env_varname_is_bound_ALT_DEF, bir_env_lookup_type_def,
-  optionTheory.IS_SOME_MAP]);
+SIMP_TAC std_ss [bir_env_varname_is_bound_ALT_DEF,
+                 bir_env_lookup_type_def,
+                 optionTheory.IS_SOME_MAP]
+);
 
 
 val bir_env_var_is_declared_def = Define `
   (bir_env_var_is_declared env v <=>
   (bir_env_lookup_type (bir_var_name v) env = SOME (bir_var_type v)))`;
 
-(* This duplication is kept deliberately, because despite the same semantics, the intentention
-   of what you want to express is different *)
-val bir_env_var_is_declared_DEF_bir_env_check_type = store_thm ("bir_env_var_is_declared_ALT_DEF",
+(* This duplication is kept deliberately, because despite the same
+ * semantics, the intention of what you want to express is
+ * different *)
+val bir_env_var_is_declared_DEF_bir_env_check_type =
+  store_thm ("bir_env_var_is_declared_ALT_DEF",
   ``bir_env_var_is_declared env v = bir_env_check_type v env``,
-SIMP_TAC std_ss [bir_env_check_type_def, bir_env_var_is_declared_def]);
+SIMP_TAC std_ss [bir_env_check_type_def,
+                 bir_env_var_is_declared_def]
+);
+*)
 
+(* Old name: bir_env_var_is_initialised *)
+val bir_env_var_is_well_typed_def = Define `
+  (bir_env_var_is_well_typed env var <=>
+    (?kv.
+      (bir_env_lookup (bir_var_name var) env = kv) /\
+      (type_of_bir_kval kv = bir_var_type var)
+    )
+  )`;
+(* No more declaration...
+val bir_env_var_is_initialised_weaken =
+  store_thm ("bir_env_var_is_initialised_weaken",
+  ``!v env.
+      bir_env_var_is_initialised env v ==>
+      bir_env_var_is_declared env v``,
 
-val bir_env_var_is_initialised_def = Define `
-  (bir_env_var_is_initialised env var <=>
-  (?v. (bir_env_lookup (bir_var_name var) env = SOME (bir_var_type var, SOME v)) /\
-       (type_of_bir_val v = SOME (bir_var_type var))))`;
-
-val bir_env_var_is_initialised_weaken = store_thm ("bir_env_var_is_initialised_weaken",
-  ``!v env. bir_env_var_is_initialised env v ==> bir_env_var_is_declared env v``,
 Cases >> SIMP_TAC std_ss [bir_env_var_is_initialised_def, bir_env_var_is_declared_def,
   GSYM LEFT_FORALL_IMP_THM, bir_env_lookup_type_def]);
+*)
+(* No more declaration...
+val bir_env_var_is_declared_weaken =
+  store_thm ("bir_env_var_is_declared_weaken",
+  ``!v env.
+      bir_env_var_is_declared env v ==>
+      bir_env_varname_is_bound env (bir_var_name v)``,
 
-
-val bir_env_var_is_declared_weaken = store_thm ("bir_env_var_is_declared_weaken",
-  ``!v env. bir_env_var_is_declared env v ==> bir_env_varname_is_bound env (bir_var_name v)``,
 Cases >> SIMP_TAC std_ss [bir_env_var_is_declared_def,
   GSYM LEFT_FORALL_IMP_THM, bir_env_varname_is_bound_ALT_DEF,
   bir_var_name_def]);
-
-
+*)
+(* TODO: Remove now? *)
 val _ = Datatype `bir_env_cond_t =
-  | BEnvCond_varname_bound string
-  | BEnvCond_var_declared bir_var_t
-  | BEnvCond_var_initialised bir_var_t`;
+  | BEnvCond_var_well_typed bir_var_t`;
 
 val bir_env_cond_eval_def = Define `
-  (bir_env_cond_eval env (BEnvCond_varname_bound vn)  <=> bir_env_varname_is_bound   env vn) /\
-  (bir_env_cond_eval env (BEnvCond_var_initialised v) <=> bir_env_var_is_initialised env v) /\
-  (bir_env_cond_eval env (BEnvCond_var_declared v)    <=> bir_env_var_is_declared    env v)`;
-
+  (bir_env_cond_eval env (BEnvCond_var_well_typed v) <=>
+    bir_env_var_is_well_typed env v)`;
 
 
 val bir_env_order_def = Define `
-  (bir_env_order env1 env2) <=> !vn. (
-     (* new vars can be added and initialised, but only of the correct type *)
+  (bir_env_order env1 env2) <=>
+    !vn. (
+(*
+     (* new vars can be added and initialised, but only of the
+      * correct type *)
      (!ty v. (bir_env_lookup vn env1 = NONE) ==>
              (bir_env_lookup vn env2 = SOME (ty, SOME v)) ==>
-             (type_of_bir_val v = SOME ty)) /\
+             (type_of_bir_val v = SOME ty)
+     ) /\
 
      (* existing vars can be initialised with the right type *)
      (!ty. (bir_env_lookup vn env1 = SOME (ty, NONE)) ==>
            (?vo. (bir_env_lookup vn env2 = SOME (ty, vo)) /\
-                 (!v. (vo = SOME v) ==> (type_of_bir_val v = SOME ty)))) /\
-
-     (* The value of existing, already initialised vars can change, but if
-        their type was OK, it stays OK. *)
-     (!ty v. (bir_env_lookup vn env1 = SOME (ty, SOME v)) ==>
-             (?v'. (bir_env_lookup vn env2 = SOME (ty, SOME v')) /\
-                   ((type_of_bir_val v = SOME ty) ==>
-                    (type_of_bir_val v' = SOME ty)))))`;
+                 (!v. (vo = SOME v) ==>
+                      (type_of_bir_val v = SOME ty)
+                 )
+           )
+     ) /\
+*)
+     (* The value of existing vars can change, but their type
+      * cannot. *)
+     (!kv ty.
+       ((bir_env_lookup vn env1 = kv) /\
+        (type_of_bir_kval kv = ty)
+       )==>
+       (?kv'.
+         ((bir_env_lookup vn env2 = kv') /\
+          (type_of_bir_kval kv' = ty)
+         )
+       )
+     )
+   )`;
 
 
 val bir_env_order_REFL = store_thm ("bir_env_order_REFL",
   ``!env. bir_env_order env env``,
-SIMP_TAC std_ss [bir_env_order_def]);
+
+SIMP_TAC std_ss [bir_env_order_def]
+);
 
 
 val bir_env_order_TRANS = store_thm ("bir_env_order_TRANS",
   ``!env1 env2 env3.
-       bir_env_order env1 env2 ==> bir_env_order env2 env3 ==>
-       bir_env_order env1 env3``,
+      bir_env_order env1 env2 ==>
+      bir_env_order env2 env3 ==>
+      bir_env_order env1 env3``,
 
-REPEAT STRIP_TAC >>
-FULL_SIMP_TAC std_ss [bir_env_order_def] >>
-GEN_TAC >>
-REPEAT (Q.PAT_X_ASSUM `!vn. P vn` (MP_TAC o Q.SPEC `vn`)) >>
-REPEAT STRIP_TAC >> FULL_SIMP_TAC std_ss [] >> REV_FULL_SIMP_TAC std_ss [] >- (
-  Cases_on `bir_env_lookup vn env2` >> FULL_SIMP_TAC std_ss [] >>
-  rename1 `bir_env_lookup _ _ = SOME xx` >>
-  Cases_on `xx` >> FULL_SIMP_TAC std_ss [] >>
-  rename1 `bir_env_lookup _ _ = SOME (ty', vo')` >>
-  Cases_on `vo'` >> FULL_SIMP_TAC std_ss []
-) >- (
-  Cases_on `vo` >> FULL_SIMP_TAC std_ss []
-));
+METIS_TAC [bir_env_order_def]
+);
 
-
-val bir_env_varname_is_bound_ORDER = store_thm ("bir_env_varname_is_bound_ORDER",
-  ``!env1 env2 v. bir_env_order env1 env2 ==>
-                  bir_env_varname_is_bound env1 v ==>
-                  bir_env_varname_is_bound env2 v``,
+(* All varnames are bound...
+val bir_env_varname_is_bound_ORDER =
+  store_thm ("bir_env_varname_is_bound_ORDER",
+  ``!env1 env2 v.
+      bir_env_order env1 env2 ==>
+      bir_env_varname_is_bound env1 v ==>
+      bir_env_varname_is_bound env2 v``,
 SIMP_TAC (std_ss++QI_ss) [bir_env_varname_is_bound_ALT_DEF, bir_env_order_def,
   bir_env_lookup_type_def, optionTheory.IS_SOME_EXISTS] >>
 REPEAT STRIP_TAC >>
@@ -303,8 +375,8 @@ ASM_SIMP_TAC std_ss [] >>
 Cases_on `vo` >> (
   SIMP_TAC std_ss [GSYM LEFT_FORALL_IMP_THM]
 ));
-
-
+*)
+(* No more declare...
 val bir_env_var_is_declared_ORDER = store_thm ("bir_env_var_is_declared_ORDER",
   ``!env1 env2 v. bir_env_order env1 env2 ==>
                   bir_env_var_is_declared env1 v ==>
@@ -319,73 +391,91 @@ ASM_SIMP_TAC std_ss [] >>
 Cases_on `vo` >> (
   SIMP_TAC std_ss [GSYM LEFT_FORALL_IMP_THM]
 ));
+*)
 
+val bir_env_var_is_well_typed_ORDER =
+  store_thm ("bir_env_var_is_well_typed_ORDER",
+  ``!env1 env2 v.
+      bir_env_order env1 env2 ==>
+      bir_env_var_is_well_typed env1 v ==>
+      bir_env_var_is_well_typed env2 v``,
 
-val bir_env_var_is_initialised_ORDER = store_thm ("bir_env_var_is_initialised_ORDER",
-  ``!env1 env2 v. bir_env_order env1 env2 ==>
-                  bir_env_var_is_initialised env1 v ==>
-                  bir_env_var_is_initialised env2 v``,
-Cases_on `v` >>
-SIMP_TAC (std_ss) [bir_env_var_is_initialised_def, bir_env_order_def,
-  optionTheory.IS_SOME_EXISTS] >>
-REPEAT STRIP_TAC >>
-rename1 `bir_env_lookup vn env1 = SOME (ty, SOME v)` >>
-Q.PAT_X_ASSUM `!vn. _` (MP_TAC o Q.SPEC `vn`) >>
-ASM_SIMP_TAC std_ss [] >>
-METIS_TAC[]);
+SIMP_TAC std_ss [bir_env_var_is_well_typed_def,
+                 bir_env_order_def]
+);
 
 
 val bir_env_cond_eval_ORDER = store_thm ("bir_env_cond_eval_ORDER",
-  ``!env1 env2 c. bir_env_order env1 env2 ==>
-                  bir_env_cond_eval env1 c ==>
-                  bir_env_cond_eval env2 c``,
+  ``!env1 env2 c.
+      bir_env_order env1 env2 ==>
+      bir_env_cond_eval env1 c ==>
+      bir_env_cond_eval env2 c``,
 
 Cases_on `c` >> (
   SIMP_TAC std_ss [bir_env_cond_eval_def] >>
-  METIS_TAC[bir_env_varname_is_bound_ORDER,
-            bir_env_var_is_declared_ORDER,
-            bir_env_var_is_initialised_ORDER]
-));
+  METIS_TAC[bir_env_var_is_well_typed_ORDER]
+)
+);
 
 
-val bir_env_vars_are_initialised_def = Define `
-  bir_env_vars_are_initialised env vs <=>
-  (!v. v IN vs ==> bir_env_var_is_initialised env v)`;
+val bir_env_vars_are_well_typed_def = Define `
+  bir_env_vars_are_well_typed env vs <=>
+    (!v. v IN vs ==> bir_env_var_is_well_typed env v)`;
 
-val bir_env_vars_are_initialised_EMPTY = store_thm ("bir_env_vars_are_initialised_EMPTY",
-  ``!env. bir_env_vars_are_initialised env {}``,
-SIMP_TAC std_ss [bir_env_vars_are_initialised_def, NOT_IN_EMPTY]);
+val bir_env_vars_are_well_typed_EMPTY =
+  store_thm ("bir_env_vars_are_well_typed_EMPTY",
+  ``!env. bir_env_vars_are_well_typed env {}``,
 
-val bir_env_vars_are_initialised_INSERT = store_thm ("bir_env_vars_are_initialised_INSERT",
-  ``!env v vs. bir_env_vars_are_initialised env (v INSERT vs) <=>
-               (bir_env_var_is_initialised env v /\ bir_env_vars_are_initialised env vs)``,
-SIMP_TAC std_ss [bir_env_vars_are_initialised_def, IN_INSERT] >>
-METIS_TAC[]);
+SIMP_TAC std_ss [bir_env_vars_are_well_typed_def, NOT_IN_EMPTY]
+);
 
-val bir_env_vars_are_initialised_UNION = store_thm ("bir_env_vars_are_initialised_UNION",
-  ``!env vs1 vs2. bir_env_vars_are_initialised env (vs1 UNION vs2) <=>
-                  (bir_env_vars_are_initialised env vs1 /\
-                   bir_env_vars_are_initialised env vs2) ``,
-SIMP_TAC std_ss [bir_env_vars_are_initialised_def, IN_UNION] >>
-METIS_TAC[]);
+val bir_env_vars_are_well_typed_INSERT =
+  store_thm ("bir_env_vars_are_well_typed_INSERT",
+  ``!env v vs.
+      bir_env_vars_are_well_typed env (v INSERT vs) <=>
+        (bir_env_var_is_well_typed env v /\
+         bir_env_vars_are_well_typed env vs
+        )``,
 
-val bir_env_vars_are_initialised_SUBSET = store_thm ("bir_env_vars_are_initialised_SUBSET",
-  ``!env vs1 vs2. bir_env_vars_are_initialised env vs1 ==>
-                  (vs2 SUBSET vs1) ==>
-                   bir_env_vars_are_initialised env vs2``,
-SIMP_TAC std_ss [bir_env_vars_are_initialised_def, SUBSET_DEF] >>
-METIS_TAC[]);
+SIMP_TAC std_ss [bir_env_vars_are_well_typed_def, IN_INSERT] >>
+METIS_TAC []
+);
+
+val bir_env_vars_are_well_typed_UNION =
+  store_thm ("bir_env_vars_are_well_typed_UNION",
+  ``!env vs1 vs2.
+      bir_env_vars_are_well_typed env (vs1 UNION vs2) <=>
+        (bir_env_vars_are_well_typed env vs1 /\
+         bir_env_vars_are_well_typed env vs2) ``,
+
+SIMP_TAC std_ss [bir_env_vars_are_well_typed_def, IN_UNION] >>
+METIS_TAC []
+);
+
+val bir_env_vars_are_well_typed_SUBSET =
+  store_thm ("bir_env_vars_are_well_typed_SUBSET",
+  ``!env vs1 vs2.
+      bir_env_vars_are_well_typed env vs1 ==>
+      (vs2 SUBSET vs1) ==>
+      bir_env_vars_are_well_typed env vs2``,
+
+SIMP_TAC std_ss [bir_env_vars_are_well_typed_def, SUBSET_DEF] >>
+METIS_TAC []
+);
 
 
-val bir_env_vars_are_initialised_ORDER = store_thm ("bir_env_vars_are_initialised_ORDER",
-  ``!env1 env2 vs. bir_env_order env1 env2 ==>
-                   bir_env_vars_are_initialised env1 vs ==>
-                   bir_env_vars_are_initialised env2 vs``,
+val bir_env_vars_are_well_typed_ORDER =
+  store_thm ("bir_env_vars_are_well_typed_ORDER",
+  ``!env1 env2 vs.
+      bir_env_order env1 env2 ==>
+      bir_env_vars_are_well_typed env1 vs ==>
+      bir_env_vars_are_well_typed env2 vs``,
 
-SIMP_TAC std_ss [bir_env_vars_are_initialised_def] >>
-METIS_TAC[bir_env_var_is_initialised_ORDER]);
+SIMP_TAC std_ss [bir_env_vars_are_well_typed_def] >>
+METIS_TAC [bir_env_var_is_well_typed_ORDER]
+);
 
-
+(* Nonsensical with new changes?
 val bir_env_order_update = store_thm ("bir_env_order_update",
 ``!env env' vn vo ty.
     ~(bir_env_varname_is_bound env vn) /\
@@ -400,7 +490,7 @@ FULL_SIMP_TAC (std_ss++boolSimps.LIFT_COND_ss++QI_ss) [
   bir_env_lookup_def, bir_env_order_def,
   FLOOKUP_UPDATE] >>
 METIS_TAC[]);
-
+*)
 
 val bir_env_order_write = store_thm ("bir_env_order_write",
 ``!env env' v va.
@@ -408,17 +498,25 @@ val bir_env_order_write = store_thm ("bir_env_order_write",
     bir_env_order env env'``,
 
 Cases >>
-SIMP_TAC (std_ss++boolSimps.LIFT_COND_ss) [bir_env_write_def, bir_env_update_def,
-  bir_env_order_def, FLOOKUP_UPDATE, bir_env_lookup_def,
-  bir_env_check_type_def, bir_env_lookup_type_def,
-  PULL_EXISTS] >>
-SIMP_TAC (std_ss++QI_ss) []);
+SIMP_TAC (std_ss++boolSimps.LIFT_COND_ss)
+         [bir_env_write_def, bir_env_update_def,
+          bir_env_order_def, bir_env_lookup_def,
+          bir_env_check_type_def, bir_env_lookup_type_def,
+          PULL_EXISTS] >>
 
+REPEAT STRIP_TAC >>
+Cases_on `bir_var_name v = vn` >> (
+  FULL_SIMP_TAC std_ss [combinTheory.UPDATE_APPLY]
+)
+);
 
-val bir_env_order_well_typed = store_thm ("bir_env_order_well_typed",
-``!env env'. bir_is_well_typed_env env ==>
-             bir_env_order env env' ==>
-             bir_is_well_typed_env env'``,
+(* Deprecated...
+val bir_env_order_well_typed =
+  store_thm ("bir_env_order_well_typed",
+  ``!env env'.
+      bir_is_well_typed_env env ==>
+      bir_env_order env env' ==>
+      bir_is_well_typed_env env'``,
 
 Cases >> Cases >>
 rename1 `bir_env_order (BEnv env_f) (BEnv env_f')` >>
@@ -437,18 +535,23 @@ Cases_on `FLOOKUP env_f vn` >- (
 rename1 `FLOOKUP env_f vn = SOME (XXX)` >> Cases_on `XXX` >>
 rename1 `FLOOKUP env_f vn = SOME (ty', vo)` >>
 ASM_SIMP_TAC std_ss [] >>
-Cases_on `vo` >> SIMP_TAC std_ss []);
+Cases_on `vo` >> SIMP_TAC std_ss []
+);
+*)
 
-
-
-(* domains *)
-
-val bir_env_domain_def = Define `bir_env_domain (BEnv env) = FDOM env`;
+(* Domains and subenvironment don't really makes sense with total
+ * maps... *)
+(* Domains *)
+(*
+val bir_env_domain_def = Define `
+  bir_env_domain (BEnv env) = FDOM env`;
 
 val bir_env_domain_FINITE = store_thm ("bir_env_domain_FINITE",
-``!env. FINITE (bir_env_domain env)``,
+  ``!env. FINITE (bir_env_domain env)``,
+
 Cases >>
-SIMP_TAC std_ss [bir_env_domain_def, FDOM_FINITE])
+SIMP_TAC std_ss [bir_env_domain_def, FDOM_FINITE]
+);
 
 
 val bir_env_domain_LOOKUP = store_thm ("bir_env_domain_LOOKUP",
@@ -456,10 +559,11 @@ val bir_env_domain_LOOKUP = store_thm ("bir_env_domain_LOOKUP",
 
 Cases >> GEN_TAC >>
 SIMP_TAC (std_ss++boolSimps.LIFT_COND_ss) [bir_env_domain_def, bir_env_lookup_def, FLOOKUP_DEF]);
+*)
 
 
-
-(* subenvironments *)
+(* Subenvironments *)
+(*
 val bir_is_subenv_def = Define `bir_is_subenv (BEnv env1) (BEnv env2) <=> (env1 SUBMAP env2)`;
 
 val bir_is_subenv_EMPTY = store_thm ("bir_is_subenv_EMPTY",
@@ -502,14 +606,20 @@ val bir_is_subenv_LOOKUP = store_thm ("bir_is_subenv_LOOKUP",
 Cases >> Cases >> GEN_TAC >>
 SIMP_TAC std_ss [bir_is_subenv_def, bir_env_domain_def, bir_env_lookup_def,
   SUBMAP_DEF, FLOOKUP_DEF])
+*)
+val bir_env_read_EQ_lookup_IMPL =
+  store_thm ("bir_env_read_EQ_lookup_IMPL",
+  ``!env1 env2 v.
+      (bir_env_lookup (bir_var_name v) env1 =
+        bir_env_lookup (bir_var_name v) env2) ==>
+      (bir_env_read v env1 = bir_env_read v env2)``,
 
-val bir_env_read_EQ_lookup_IMPL = store_thm ("bir_env_read_EQ_lookup_IMPL",
-``!env1 env2 v.
-   (bir_env_lookup (bir_var_name v) env1 = bir_env_lookup (bir_var_name v) env2) ==>
-   (bir_env_read v env1 = bir_env_read v env2)``,
-SIMP_TAC std_ss [bir_env_read_def]);
+SIMP_TAC std_ss [bir_env_read_def,
+                 bir_env_check_type_def,
+                 bir_env_lookup_type_def]
+);
 
-
+(*
 val bir_is_subenv_READ = store_thm ("bir_is_subenv_READ",
   ``!env1 env2 v.
        bir_is_subenv env1 env2 ==>
@@ -517,57 +627,98 @@ val bir_is_subenv_READ = store_thm ("bir_is_subenv_READ",
        (bir_env_read v env1 = bir_env_read v env2)``,
 
 SIMP_TAC std_ss [bir_env_read_def] >>
-METIS_TAC[bir_is_subenv_LOOKUP]);
-
+METIS_TAC [bir_is_subenv_LOOKUP]);
+*)
 
 
 (* Equivalence for sets of vars *)
 val bir_env_EQ_FOR_VARS_def = Define `
   bir_env_EQ_FOR_VARS vs env1 env2 <=>
-  (!v. v IN vs ==> (bir_env_lookup (bir_var_name v) env1 = bir_env_lookup (bir_var_name v) env2))`
+    (!v.
+      v IN vs ==>
+      (bir_env_lookup (bir_var_name v) env1 =
+        bir_env_lookup (bir_var_name v) env2
+      )
+    )`
 
-val bir_env_EQ_FOR_VARS_EQUIV_EQ = store_thm ("bir_env_EQ_FOR_VARS_EQUIV_EQ",
-  ``!vs env1 env2. (bir_env_EQ_FOR_VARS vs env1 env2) <=>
-                   (bir_env_EQ_FOR_VARS vs env1 = bir_env_EQ_FOR_VARS vs env2)``,
+val bir_env_EQ_FOR_VARS_EQUIV_EQ =
+  store_thm ("bir_env_EQ_FOR_VARS_EQUIV_EQ",
+  ``!vs env1 env2.
+      (bir_env_EQ_FOR_VARS vs env1 env2) <=>
+        (bir_env_EQ_FOR_VARS vs env1 =
+          bir_env_EQ_FOR_VARS vs env2
+        )``,
 
 SIMP_TAC std_ss [bir_env_EQ_FOR_VARS_def, FUN_EQ_THM] >>
-METIS_TAC[]);
+METIS_TAC []
+);
 
 
-val bir_env_EQ_FOR_VARS_EQUIV = store_thm ("bir_env_EQ_FOR_VARS_EQUIV",
+val bir_env_EQ_FOR_VARS_EQUIV =
+  store_thm ("bir_env_EQ_FOR_VARS_EQUIV",
  ``(!vs env. bir_env_EQ_FOR_VARS vs env env) /\
-   (!vs env1 env2. (bir_env_EQ_FOR_VARS vs env1 env2 <=> (bir_env_EQ_FOR_VARS vs env2 env1))) /\
-   (!vs env1 env2 env3. bir_env_EQ_FOR_VARS vs env1 env2 ==>
-                        bir_env_EQ_FOR_VARS vs env2 env3 ==>
-                        bir_env_EQ_FOR_VARS vs env1 env3)``,
-SIMP_TAC std_ss [bir_env_EQ_FOR_VARS_def] >> METIS_TAC[]);
+   (!vs env1 env2.
+     (bir_env_EQ_FOR_VARS vs env1 env2 <=>
+       (bir_env_EQ_FOR_VARS vs env2 env1)
+     )
+   ) /\
+   (!vs env1 env2 env3.
+     bir_env_EQ_FOR_VARS vs env1 env2 ==>
+     bir_env_EQ_FOR_VARS vs env2 env3 ==>
+     bir_env_EQ_FOR_VARS vs env1 env3
+   )``,
 
-
-
-val bir_env_EQ_FOR_VARS_EMPTY = store_thm ("bir_env_EQ_FOR_VARS_EMPTY",
-  ``!env1 env2. bir_env_EQ_FOR_VARS EMPTY env1 env2``,
-SIMP_TAC std_ss [bir_env_EQ_FOR_VARS_def, NOT_IN_EMPTY, bir_env_EQ_FOR_VARS_def]);
-
-
-val bir_env_EQ_FOR_VARS_UNIV = store_thm ("bir_env_EQ_FOR_VARS_UNIV",
-  ``!env1 env2. bir_env_EQ_FOR_VARS UNIV env1 env2 <=> (env1 = env2)``,
-REPEAT Cases >>
-SIMP_TAC (std_ss++DatatypeSimps.expand_type_quants_ss [``:bir_var_t``]) [
-  bir_env_EQ_FOR_VARS_def, IN_UNIV, FLOOKUP_EXT,
-  bir_var_environment_t_11, bir_env_lookup_def, bir_var_name_def, FUN_EQ_THM]);
-
-
-val bir_env_EQ_FOR_VARS_SUBSET = store_thm ("bir_env_EQ_FOR_VARS_SUBSET",
-  ``!vs1 vs2 env1 env2. vs2 SUBSET vs1 ==> bir_env_EQ_FOR_VARS vs1 env1 env2 ==> bir_env_EQ_FOR_VARS vs2 env1 env2``,
-SIMP_TAC std_ss [bir_env_EQ_FOR_VARS_def, SUBSET_DEF] >>
-METIS_TAC[]);
-
-
-val bir_env_EQ_FOR_VARS_read_IMPL = store_thm ("bir_env_EQ_FOR_VARS_read_IMPL",
-``!vs env1 env2. bir_env_EQ_FOR_VARS vs env1 env2 ==>
-  (!v. v IN vs ==> (bir_env_read v env1 = bir_env_read v env2))``,
 SIMP_TAC std_ss [bir_env_EQ_FOR_VARS_def] >>
-METIS_TAC[bir_env_read_EQ_lookup_IMPL]);
+METIS_TAC []
+);
+
+
+
+val bir_env_EQ_FOR_VARS_EMPTY =
+  store_thm ("bir_env_EQ_FOR_VARS_EMPTY",
+  ``!env1 env2. bir_env_EQ_FOR_VARS EMPTY env1 env2``,
+
+SIMP_TAC std_ss [bir_env_EQ_FOR_VARS_def, NOT_IN_EMPTY,
+                 bir_env_EQ_FOR_VARS_def]
+);
+
+
+val bir_env_EQ_FOR_VARS_UNIV =
+  store_thm ("bir_env_EQ_FOR_VARS_UNIV",
+  ``!env1 env2.
+      bir_env_EQ_FOR_VARS UNIV env1 env2 <=> (env1 = env2)``,
+
+REPEAT Cases >>
+SIMP_TAC (std_ss++DatatypeSimps.expand_type_quants_ss[``:bir_var_t``]) [bir_env_EQ_FOR_VARS_def, IN_UNIV,
+    bir_var_environment_t_11, bir_env_lookup_def, bir_var_name_def,
+    FUN_EQ_THM]
+);
+
+
+val bir_env_EQ_FOR_VARS_SUBSET =
+  store_thm ("bir_env_EQ_FOR_VARS_SUBSET",
+  ``!vs1 vs2 env1 env2.
+      vs2 SUBSET vs1 ==>
+      bir_env_EQ_FOR_VARS vs1 env1 env2 ==>
+      bir_env_EQ_FOR_VARS vs2 env1 env2``,
+
+SIMP_TAC std_ss [bir_env_EQ_FOR_VARS_def, SUBSET_DEF] >>
+METIS_TAC []
+);
+
+
+val bir_env_EQ_FOR_VARS_read_IMPL =
+  store_thm ("bir_env_EQ_FOR_VARS_read_IMPL",
+  ``!vs env1 env2.
+      bir_env_EQ_FOR_VARS vs env1 env2 ==>
+      (!v.
+        v IN vs ==>
+        (bir_env_read v env1 = bir_env_read v env2)
+      )``,
+
+SIMP_TAC std_ss [bir_env_EQ_FOR_VARS_def] >>
+METIS_TAC [bir_env_read_EQ_lookup_IMPL]
+);
 
 
 val _ = export_theory();
